\section{Matrix Inverse Formulas}
This chapter contains formulas for the inverses of various sums of matrices.

\subsection{Inverse of $A+B$}
Let $C+D$ be the inverse of $A+B$, then
\begin{align}
(C+D)(A+B) &= I \nonumber \\
\Rightarrow CA + CB + DA + DB &= I.
\end{align}
Now let $C=A^{-1}$, then
\begin{align}
A^{-1}A + A^{-1}B + DA + DB & = I \nonumber \\
\Rightarrow A^{-1}B + DA + DB & = 0.
\end{align}
Now let $D=A^{-1}MA^{-1}$, then
\begin{align}
A^{-1}B + A^{-1}M + A^{-1}MA^{-1}B & = 0 \nonumber \\
\Rightarrow A^{-1}\left(B + M + MA^{-1}B\right) &= 0 \nonumber \\
\Rightarrow B + M + MA^{-1}B & = 0.
\end{align}
Now let $M=BFB$, then
\begin{align}
B + BFB + BFBA^{-1}B & = 0 \nonumber \\
\Rightarrow B\left(I + FB + FBA^{-1}B\right) &= 0 \nonumber \\
\Rightarrow I+FB+FBA^{-1}B & = 0 \nonumber \\
\Rightarrow F(B+BA^{-1}B) &= -I \nonumber \\
\Rightarrow F &= (B+BA^{-1}B)^{-1}.
\end{align}
Therefore $D=A^{-1}B(B+BA^{-1}B)^{-1}BA^{-1}$. Substituting for $C$ and $D$, the inverse of $A+B$ is then
\begin{equation}
(A+B)^{-1} = A^{-1} - A^{-1}B(B+BA^{-1}B)^{-1}BA^{-1}
\label{linalg:invaplusb}
\end{equation}
Note that \eqref{linalg:invaplusb} only requires $A$ to be invertible. If $B$ is invertible \eqref{linalg:invaplusb} can be simplified to
\begin{equation}
(A+B)^{-1} = A^{-1} - A^{-1}B(I+A^{-1}B)^{-1}A^{-1}
\end{equation}
or
\begin{equation}
(A+B)^{-1} = A^{-1} - A^{-1}(I+BA^{-1})BA^{-1}
\end{equation}

\subsection{Inverse of $A+BCD$}
Using \eqref{linalg:invaplusb}
\begin{align}
(A+BCD)^{-1} &= A^{-1}-A^{-1}BCD(BCD + BCDA^{-1}BCD)^{-1}BCDA^{-1} \nonumber \\
&= A^{-1} + A^{-1}BCD(BC(D+DA^{-1}BCD))^{-1}BCDA^{-1} \nonumber \\
&= A^{-1} + A^{-1}BCD(D+DA^{-1}BCD)DA^{-1} \nonumber \\
&= A^{-1} + A^{-1}BCD((D(CD)^{-1}+DA^{-1}B)CD)^{-1}DA^{-1} \nonumber \\
&= A^{-1} + A^{-1}B(C^{-1} + DA^{-1}B)^{-1}DA^{-1}
\end{align}

\subsection{Inverse of $AB+CD$}
Using \eqref{linalg:invaplusb}
\begin{align}
(AB+CD)^{-1} &= B^{-1}A^{-1} - (AB)^{-1}CD(CD+CD(AB)^{-1}CD)^{-1}CD(AB)^{-1} \nonumber \\
&= B^{-1}A^{-1} - B^{-1}A^{-1}CD(CD(I+(AB)^{-1}CD))^{-1}CDB^{-1}A^{-1} \nonumber \\
&= B^{-1}A^{-1} - B^{-1}A^{-1}CD(I+B^{-1}A^{-1}CD)^{-1}B^{-1}A^{-1}
\end{align}